theories/instructions/stp_test.v
@@ -10,10 +10,10 @@ Definition sys_regs `{!islaG Σ} `{!threadG} : iProp Σ :=
   ("SCTLR_EL2" ↦ᵣ Val_Bits [BV{64} 0x0000000004000002] ∗
   "SCR_EL3" ↦ᵣ Val_Bits [BV{32} 0] ∗
   "TCR_EL2" ↦ᵣ Val_Bits [BV{64} 0] ∗
-  "CFG_ID_AA64PFR0_EL1_EL0" ↦ᵣ Val_Bits [BV{1} 1] ∗
-  "CFG_ID_AA64PFR0_EL1_EL1" ↦ᵣ Val_Bits [BV{1} 1] ∗
-  "CFG_ID_AA64PFR0_EL1_EL2" ↦ᵣ Val_Bits [BV{1} 1] ∗
-  "CFG_ID_AA64PFR0_EL1_EL3" ↦ᵣ Val_Bits [BV{1} 1] ∗
+  "CFG_ID_AA64PFR0_EL1_EL0" ↦ᵣ Val_Bits [BV{4} 1] ∗
+  "CFG_ID_AA64PFR0_EL1_EL1" ↦ᵣ Val_Bits [BV{4} 1] ∗
+  "CFG_ID_AA64PFR0_EL1_EL2" ↦ᵣ Val_Bits [BV{4} 1] ∗
+  "CFG_ID_AA64PFR0_EL1_EL3" ↦ᵣ Val_Bits [BV{4} 1] ∗
   "OSLSR_EL1" ↦ᵣ Val_Bits [BV{32} 0] ∗
   "OSDLR_EL1" ↦ᵣ Val_Bits [BV{32} 0] ∗
   "EDSCR" ↦ᵣ Val_Bits [BV{32} 0] ∗
@@ -31,25 +31,43 @@ Definition sys_regs `{!islaG Σ} `{!threadG} : iProp Σ :=
           ("SSBS", Val_Poison); ("T", Val_Poison); ("J", Val_Poison);
           ("V", Val_Bits [BV{1} 0]); ("DIT", Val_Bits [BV{1} 0])]))%I.
 
+Definition cont_spec `{!islaG Σ} `{!threadG} a sp (v1 v2 : bv 64) : iProp Σ :=
+  ∃ (vold1 vold2 : bv 64),
+  "R0" ↦ᵣ Val_Bits v1 ∗
+  "R1" ↦ᵣ Val_Bits v2 ∗
+  (bv_sub sp [BV{64} 16]) ↦ₘ vold1 ∗
+  (bv_sub sp [BV{64} 8]) ↦ₘ vold2 ∗
+  (*⌜(bv_and sp [BV{64} 0xFFF0000000000000]) = [BV{64} 0]⌝ ∗ *)
+  ⌜top_bits_zero 12 sp⌝ ∗
+  "SP_EL2" ↦ᵣ Val_Bits sp ∗
+  sys_regs ∗
+  instr_pre a (
+    "R0" ↦ᵣ Val_Bits v1 ∗
+    "R1" ↦ᵣ Val_Bits v2 ∗
+    "SP_EL2" ↦ᵣ Val_Bits (bv_sub sp [BV{64} 16])∗
+    sys_regs ∗
+    (bv_sub sp [BV{64} 16]) ↦ₘ v1 ∗
+    (bv_sub sp [BV{64} 8]) ↦ₘ v2 ∗
+    True).
 
-Lemma stp_wp `{!islaG Σ} `{!threadG} (sp : bv 64):
+Lemma mod_inj a b c d n (P1: a `mod` n = c `mod` n) (P2 : b `mod` n = d `mod` n) : (a + b) `mod` n = (c + d) `mod` n.
+Proof.
+  destruct (Z.eq_dec 0 n).
+  + destruct e.
+    by repeat rewrite Zmod_0_r.
+  + rewrite (Z.add_mod a b); [|done].
+    rewrite (Z.add_mod c d); [|done].
+    by rewrite P1 P2.
+Qed.
+
+Lemma stp_wp `{!islaG Σ} `{!threadG} (sp v1 v2: bv 64):
   instr 0x0000000010300000 (Some [stp_trace]) -∗
-  (*instr 0x0000000010300004 None -∗ *)
-  "_PC" ↦ᵣ Val_Bits start_address -∗
-  "__PC_changed" ↦ᵣ Val_Bool false -∗
-  "R0" ↦ᵣ Val_Bits [BV{64} 0x0000000000000400] -∗
-  "R1" ↦ᵣ Val_Bits [BV{64} 0x0000000000000200] -∗
-  sp ↦ₘ [BV{64} 0x0000000000000002] -∗
-  (bv_sub sp [BV{64} 16]) ↦ₘ [BV{64} 0x0000000000000001] -∗
-  "SP_EL2" ↦ᵣ Val_Bits sp -∗
-  sys_regs -∗
-  spec_trace spec -∗
-  ("_PC" ↦ᵣ Val_Bits (bv_add start_address [BV{64} 4]) -∗ "__PC_changed" ↦ᵣ Val_Bool false -∗ WPasm []) -∗
-  WPasm [].
+  instr_body 0x0000000010300000 (cont_spec 0x0000000010300004 sp v1 v2).
 Proof.
     iStartProof.
-    unfold sys_regs.
+    unfold cont_spec, sys_regs.
     repeat liAStep; liShow.
     Unshelve.
-    done.
+    all: try done.
+    all: try (repeat f_equal; unLET; bv_solve).
 Qed.
